progress in Cligtgenproof

rustfrontend/Clightgenproof.v
@@ -14,12 +14,14 @@ Require Import LanguageInterface cklr.CKLR cklr.Inject cklr.InjectFootprint.
 
 Import ListNotations.
 
+Local Open Scope error_monad_scope.
+Local Open Scope gensym_monad_scope.
+
 (** Correctness proof for the generation of Clight *)
 
-
 Record match_prog (p: RustIR.program) (tp: Clight.program) : Prop := {
-    match_prog_types:
-    tp.(Ctypes.prog_types) = transl_composites p.(prog_types);
+    match_prog_comp_env:
+    tr_composite_env p.(prog_comp_env) tp.(Ctypes.prog_comp_env);
     match_prog_def:    
     match_program_gen tr_fundef (fun ty ty' => to_ctype ty = ty') p p tp;
     match_prog_skel:
@@ -28,16 +30,15 @@ Record match_prog (p: RustIR.program) (tp: Clight.program) : Prop := {
 
 Section PRESERVATION.
 
-Variable match_prog: RustIR.program -> Clight.program -> Prop. (* TODO *)
-
 Variable prog: RustIR.program.
 Variable tprog: Clight.program.
-Hypothesis TRANSL: match_prog  prog tprog.
+Hypothesis TRANSL: match_prog prog tprog.
 
 Variable se: Genv.symtbl.
 Variable tse: Genv.symtbl.
 (* injp or inj ? *)
-Variable w: world injp.
+
+Variable w: inj_world.
 Let ge := RustIR.globalenv se prog.
 Let tge := Clight.globalenv tse tprog.
 
@@ -64,65 +65,61 @@ Inductive match_cont : RustIR.cont -> Clight.cont -> Prop :=
     tr_stmt ce tce dropm s ts ->
     match_cont k tk ->
     match_cont (RustIR.Kloop s k) (Clight.Kloop1 ts Clight.Sskip tk)
-| match_Kcall1: forall p f tf e te le k tk cty temp pe,
+| match_Kcall1: forall p f tf e te le k tk cty temp pe j,
     (* we need to consider temp is set to a Clight expr which is
     translated from p *)
     transl_function ce tce dropm f = OK tf ->
     cty = to_ctype (typeof_place p) ->
     place_to_cexpr tce p = OK pe ->
     match_cont k tk ->
-    match_env (mi injp w) e te ->
+    match_env j e te ->
     match_cont (RustIR.Kcall (Some p) f e k) (Clight.Kcall (Some temp) tf te le (Clight.Kseq (Clight.Sassign pe (Etempvar temp cty)) tk))
 | match_Kcall2: forall f tf e te le k tk,
     (* how to relate le? *)
     transl_function ce tce dropm f = OK tf ->
     match_cont k tk ->
     match_cont (RustIR.Kcall None f e k) (Clight.Kcall None tf te le tk)
-| match_Kcalldrop: forall id e te le k tk tf co,
+| match_Kcalldrop: forall id e te le k tk tf co j,
     (* Is it correct? *)
     ce ! id = Some co ->
-    drop_glue_for_composite ce tce dropm id co.(co_sv) co.(co_members) co.(co_attr)= OK (Some tf) ->
-    match_env (mi injp w) e te ->
+    drop_glue_for_composite ce tce dropm id co.(co_sv) co.(co_members) co.(co_attr) = OK (Some tf) ->
+    match_env j e te ->
     match_cont (RustIR.Kcalldrop id e k) (Clight.Kcall None tf te le tk)
 .
 
 
 Inductive match_states: RustIR.state -> Clight.state -> Prop :=
-| match_regular_state: forall f tf s ts k tk m tm e te le j Hm,
-    (* Ignore the generators here *)
-    transl_function ce tce dropm f = OK tf ->
-    tr_stmt ce tce dropm s ts ->
+| match_regular_state: forall f tf s ts k tk m tm e te le j
+    (MFUN: tr_function ce tce dropm f tf)
+    (MSTMT: tr_stmt ce tce dropm s ts)
     (* match continuation *)
-    match_cont k tk ->
-    (* we need to consider that tm may contains more block for its call stacks of drop glue *)
-    (* use injp_acc ? *)
-    injp_acc w (injpw j m tm Hm) ->
-    (* local environments are the same? *)
-    match_env (mi injp w) e te ->
+    (MCONT: match_cont k tk)
+    (MINJ: Mem.inject j m tm)   
+    (MENV: match_env j e te),
     match_states (RustIR.State f s k e m) (Clight.State tf ts tk te le tm)
-| match_call_state: forall vf vargs k m tvf tvargs tk tm j fd targs tres cconv Hm orgs rels
+| match_call_state: forall vf vargs k m tvf tvargs tk tm j fd targs tres cconv orgs rels
    (MCONT: match_cont k tk)
    (VINJ: Val.inject j vf tvf)
-   (MINJ: injp_acc w (injpw j m tm Hm))
+   (MINJ: Mem.inject j m tm)
    (AINJ: Val.inject_list j vargs tvargs)
    (VFIND: Genv.find_funct ge vf = Some fd)
    (FUNTY: type_of_fundef fd = Tfunction orgs rels targs tres cconv),
     match_states (RustIR.Callstate vf vargs k m) (Clight.Callstate tvf tvargs tk tm)
-| match_return_state: forall v k m tv tk tm j Hm
+| match_return_state: forall v k m tv tk tm j
    (MCONT: match_cont k tk)
-   (MINJ: injp_acc w (injpw j m tm Hm))
+   (MINJ: Mem.inject j m tm)
    (RINJ: Val.inject j v tv),
     match_states (RustIR.Returnstate v k m) (Clight.Returnstate tv tk tm)
-| match_calldrop_box: forall p k e m b ofs tk tm ty a j Hm fb
+| match_calldrop_box: forall p k e m b ofs tk tm ty a j fb
     (* we can store the address of p in calldrop and build a local env
     in Drop state according to this address *)
     (VFIND: Genv.find_def tge fb = Some (Gfun malloc_decl))
     (PTY: typeof_place p = Tbox ty a)
     (PADDR: eval_place ce e m p b ofs)
     (MCONT: match_cont k tk)
-    (MINJ: injp_acc w (injpw j m tm Hm)),
+    (MINJ: Mem.inject j m tm),
     match_states (RustIR.Calldrop p k e m) (Clight.Callstate (Vptr fb Ptrofs.zero) [(Vptr b ofs)] tk tm)
-| match_calldrop_composite: forall p k e m b ofs tk tm a j Hm fb id fid drop_glue orgs
+| match_calldrop_composite: forall p k e m b ofs tk tm a j fb id fid drop_glue orgs
     (DROPM: dropm!id = Some fid)
     (VFIND: Genv.find_def tge fb = Some drop_glue)
     (SYMB: Genv.find_symbol tge fid = Some fb)
@@ -131,22 +128,100 @@ Inductive match_states: RustIR.state -> Clight.state -> Prop :=
     (PTY: typeof_place p = Tstruct orgs id a \/ typeof_place p = Tvariant orgs id a)
     (PADDR: eval_place ce e m p b ofs)
     (MCONT: match_cont k tk)
-    (MINJ: injp_acc w (injpw j m tm Hm)),
+    (MINJ: Mem.inject j m tm),
     match_states (RustIR.Calldrop p k e m) (Clight.Callstate (Vptr fb Ptrofs.zero) [(Vptr b ofs)] tk tm)
-| match_drop_state: forall id s k e m tf ts tk te le tm j Hm co
+| match_drop_state: forall id s k e m tf ts tk te le tm j co
     (* How to relate e and te? and le? *)
     (MSTMT: tr_stmt ce tce dropm s ts)
     (MCONT: match_cont k tk)
-    (MINJ: injp_acc w (injpw j m tm Hm)),
+    (MINJ: Mem.inject j m tm),
     ce ! id = Some co ->
     drop_glue_for_composite ce tce dropm id co.(co_sv) co.(co_members) co.(co_attr) = OK (Some tf) ->
     match_states (RustIR.Dropstate id s k e m) (Clight.State tf ts tk te le tm)
 .
 
+(* Type preservation in translation *)
+
+Lemma place_to_cexpr_type: forall p e,
+    place_to_cexpr tce p = OK e ->
+    Clight.typeof e = to_ctype (typeof_place p).
+Admitted.
+
+Lemma expr_to_cexpr_type: forall e e',
+    expr_to_cexpr ce tce e = OK e' ->
+    Clight.typeof e' = to_ctype (typeof e) .
+Admitted.
+
+
+(* Injection is preserved during evaluation *)
+
+Lemma eval_expr_inject: forall e te j a a' m tm v le,
+    expr_to_cexpr ce tce a = OK a' ->
+    eval_expr ge e m a v ->
+    match_env j e te ->
+    Mem.inject j m tm ->
+    exists v', Clight.eval_expr tge te le tm a' v' /\ Val.inject j v v'.
+(* To prove this lemma, we need to support type checking in the
+   evaluation of expression in RustIR *)
+Admitted.
+
+Lemma eval_place_inject: forall e te j p lv m tm le b ofs,
+    place_to_cexpr tce p = OK lv ->
+    eval_place ge e m p b ofs ->
+    match_env j e te ->
+    Mem.inject j m tm ->
+    exists b' ofs', Clight.eval_lvalue tge te le tm lv b' ofs' Full /\ Val.inject j (Vptr b ofs) (Vptr b' ofs').
+Admitted.
+
+Lemma assign_loc_inject: forall f ty m loc ofs v m' tm loc' ofs' v',
+    assign_loc ge ty m loc ofs v m' ->
+    Val.inject f (Vptr loc ofs) (Vptr loc' ofs') ->
+    Val.inject f v v' ->
+    Mem.inject f m tm ->
+    exists tm',
+      Clight.assign_loc tge (to_ctype ty) tm loc' ofs' Full v' tm'
+      /\ Mem.inject f m' tm'.
+Admitted.
+
+
 
 Lemma step_simulation:
   forall S1 t S2, step ge S1 t S2 ->
-  forall S1' (MS: match_states S1 S1'), exists S2', plus step2 tge S1' t S2' /\ match_states S2 S2'.
+  forall S1' (MS: match_states S1 S1'), exists S2', plus step1 tge S1' t S2' /\ match_states S2 S2'.
+Proof.
+  induction 1; intros; inv MS.
+  
+  (* assign *)
+  - inv MSTMT. simpl in H2.
+    monadInv_comb H2.
+    (* eval place and expr *)
+    exploit eval_place_inject;eauto. instantiate (1:= le0).
+    intros (b' & ofs' & EL & INJL).
+    exploit eval_expr_inject; eauto. instantiate (1:= le0).
+    intros (v' & ER & INJR).
+    exploit assign_loc_inject;eauto.
+    intros (tm2 & TASS & INJA).
+    eexists. split.
+    (* step *)
+    + eapply plus_one.
+      eapply Clight.step_assign;eauto.
+      (* sem_cast *)
+      instantiate (1:= v').
+      (* Proof strategy:
+         1. type equal between lhs and rhs
+         2. evaluation of well typed expression produces casted value (val_casted)
+         3. use cast_val_casted *)
+      admit.
+      (* assign_loc *)
+      erewrite place_to_cexpr_type; eauto.
+    (* match state *)
+    + eapply match_regular_state;eauto.
+      econstructor. simpl. eauto.
+
+  (* assign_variant *)
+  - inv MSTMT. simpl in H6.
+    monadInv_comb H6.
+      
 Admitted.
 
 Lemma initial_states_simulation:
